common/Values.v
@@ -21,6 +21,11 @@ Require Import AST.
 Require Import Integers.
 Require Import Floats.
 
+Definition compartment : Type := positive.
+Definition default_compartment : compartment := 1%positive.
+Definition eq_compartment (c1 c2: compartment) :=
+  peq c1 c2.
+
 Definition block : Type := positive.
 Definition eq_block := peq.
 
