backend/Stackingproof.v
@@ -1036,18 +1036,18 @@ Qed.
   saving of the used callee-save registers). *)
 
 Lemma function_prologue_correct:
-  forall j ls ls0 ls1 rs rs1 m1 m1' m2 sp parent ra cs fb k P,
+  forall j ls ls0 ls1 rs rs1 m1 c m1' m2 sp parent ra cs fb k P,
   agree_regs j ls rs ->
   agree_callee_save ls ls0 ->
   agree_outgoing_arguments (Linear.fn_sig f) ls ls0 ->
   (forall r, Val.has_type (ls (R r)) (mreg_type r)) ->
   ls1 = LTL.undef_regs destroyed_at_function_entry (LTL.call_regs ls) ->
   rs1 = undef_regs destroyed_at_function_entry rs ->
-  Mem.alloc m1 0 f.(Linear.fn_stacksize) = (m2, sp) ->
+  Mem.alloc m1 c 0 f.(Linear.fn_stacksize) = (m2, sp) ->
   Val.has_type parent Tptr -> Val.has_type ra Tptr ->
   m1' |= minjection j m1 ** globalenv_inject ge j ** P ->
   exists j', exists rs', exists m2', exists sp', exists m3', exists m4', exists m5',
-     Mem.alloc m1' 0 tf.(fn_stacksize) = (m2', sp')
+     Mem.alloc m1' c 0 tf.(fn_stacksize) = (m2', sp')
   /\ store_stack m2' (Vptr sp' Ptrofs.zero) Tptr tf.(fn_link_ofs) parent = Some m3'
   /\ store_stack m3' (Vptr sp' Ptrofs.zero) Tptr tf.(fn_retaddr_ofs) ra = Some m4'
   /\ star step tge
@@ -1067,7 +1067,7 @@ Local Opaque b fe.
   generalize (frame_env_range b) (frame_env_aligned b). replace (make_env b) with fe by auto. simpl.
   intros LAYOUT1 LAYOUT2.
   (* Allocation step *)
-  destruct (Mem.alloc m1' 0 (fe_size fe)) as [m2' sp'] eqn:ALLOC'.
+  destruct (Mem.alloc m1' c 0 (fe_size fe)) as [m2' sp'] eqn:ALLOC'.
   exploit alloc_parallel_rule_2.
   eexact SEP. eexact ALLOC. eexact ALLOC'.
   instantiate (1 := fe_stack_data fe). tauto.
